# baseURI: http://rdf.cdisc.org/cdash-1-1/schema
# imports: http://rdf.cdisc.org/schema

# c14n-version: 3
@prefix cdashs: <http://rdf.cdisc.org/cdash-1-1/schema#> .
@prefix cdiscs: <http://rdf.cdisc.org/schema#> .
@prefix dc: <http://purl.org/dc/elements/1.1/> .
@prefix mms: <http://rdf.cdisc.org/mms#> .
@prefix owl: <http://www.w3.org/2002/07/owl#> .
@prefix rdf: <http://www.w3.org/1999/02/22-rdf-syntax-ns#> .
@prefix rdfs: <http://www.w3.org/2000/01/rdf-schema#> .
@prefix skos: <http://www.w3.org/2004/02/skos/core#> .
@prefix xsd: <http://www.w3.org/2001/XMLSchema#> .
<http://rdf.cdisc.org/cdash-1-1/schema>
  rdf:type owl:Ontology ;
  dc:creator "FDA/PhUSE CSS Semantic Technology Project"^^xsd:string ;
  rdfs:label "CDASH 1.1 Schema"^^xsd:string ;
  owl:imports <http://rdf.cdisc.org/schema> ;
  owl:versionInfo "1.1"^^xsd:string ;
  skos:definition "The CDASH Schema defines additional elements that are specific to CDASH and not part of the CDISC schema."^^xsd:string ;
.
<http://rdf.cdisc.org/cdash-1-1/schema#Classifier.HighlyRecommendedField>
  rdf:type cdiscs:DataElementCompliance ;
  rdfs:label "Highly Recommended Data Collection Field"^^xsd:string ;
  skos:definition "Highly Recommended (HR): A data collection field that should be on the CRF (e.g., a regulatory requirement)."^^xsd:string ;
.
<http://rdf.cdisc.org/cdash-1-1/schema#Classifier.OptionalField>
  rdf:type cdiscs:DataElementCompliance ;
  rdfs:label "Optional Data Collection Field"^^xsd:string ;
  skos:definition "Optional (O): A data collection field that is available for use."^^xsd:string ;
.
<http://rdf.cdisc.org/cdash-1-1/schema#Classifier.RecommendedOrConditionalField>
  rdf:type cdiscs:DataElementCompliance ;
  rdfs:label "Recommended or Conditional Data Collection Field"^^xsd:string ;
  skos:definition "Recommended/Conditional (R/C): A data collection field that should be on a CRF based on certain conditions (e.g., complete date of birth is preferred, but may not be allowed in some regions; AE time should only be captured if there is another data point with which to compare it). In the absence of this data point other data points would be less meaningful."^^xsd:string ;
.
cdashs:crfCompletionInstructions
  rdf:type owl:DatatypeProperty ;
  rdfs:domain mms:DataElement ;
  rdfs:isDefinedBy <http://rdf.cdisc.org/schema> ;
  rdfs:label "CDASH CRF Completion Instructions"^^xsd:string ;
  rdfs:range xsd:string ;
.
cdashs:prompt
  rdf:type owl:DatatypeProperty ;
  rdfs:domain mms:DataElement ;
  rdfs:isDefinedBy <http://rdf.cdisc.org/schema> ;
  rdfs:label "CDASH Data Element Prompt"^^xsd:string ;
  rdfs:range xsd:string ;
  rdfs:subPropertyOf mms:dataElementLabel ;
.
cdashs:questionText
  rdf:type owl:DatatypeProperty ;
  rdfs:domain mms:DataElement ;
  rdfs:isDefinedBy <http://rdf.cdisc.org/schema> ;
  rdfs:label "CDASH Data Element Question Text"^^xsd:string ;
  rdfs:range xsd:string ;
.
